I give up on ceres. Better show instances for me.

src/coq/GenAST.v
@@ -27,67 +27,226 @@ Section ShowInstances.
   Derive Show for raw_id.
   Derive Show for ident.
 
+  Local Open Scope string.
+
   Fixpoint show_typ (t : typ) : string :=
     match t with
-    | TYPE_I sz                 => "TYPE_I " ++ show sz
-    | TYPE_Pointer t            => "TYPE_Pointer" ++ show_typ t
-    | TYPE_Void                 => "TYPE_Void"
-    | TYPE_Half                 => "TYPE_Half"
-    | TYPE_Float                => "TYPE_Float"
-    | TYPE_Double               => "TYPE_Double"
-    | TYPE_X86_fp80             => "TYPE_X86_fp80"
-    | TYPE_Fp128                => "TYPE_Fp128"
-    | TYPE_Ppc_fp128            => "TYPE_Ppc_fp128"
-    | TYPE_Metadata             => "TYPE_Metadata"
-    | TYPE_X86_mmx              => "TYPE_X86_mmx"
-    | TYPE_Array sz t           => "TYPE_Array " ++ show sz ++ " " ++ show_typ t
-    | TYPE_Function ret args    => "TYPE_Function " ++ show_typ ret ++ " (" ++ concat ", " (map show_typ args) ++ ")"
-    | TYPE_Struct fields        => "TYPE_Struct {" ++ concat ", " (map show_typ fields) ++ "}"
-    | TYPE_Packed_struct fields => "TYPE_Packed_struct {" ++ concat ", " (map show_typ fields) ++ "}"
-    | TYPE_Opaque               => "TYPE_Opaque"
-    | TYPE_Vector sz t          => "TYPE_Vector " ++ show sz ++ " " ++ show_typ t
-    | TYPE_Identified id        => "TYPE_Identified " ++ show id
+    | TYPE_I sz                 => "i" ++ show sz
+    | TYPE_Pointer t            => show_typ t ++ "*"
+    | TYPE_Void                 => "void"
+    | TYPE_Half                 => "half"
+    | TYPE_Float                => "float"
+    | TYPE_Double               => "double"
+    | TYPE_X86_fp80             => "x86_fp80"
+    | TYPE_Fp128                => "fp128"
+    | TYPE_Ppc_fp128            => "ppc_fp128"
+    | TYPE_Metadata             => "metadata"
+    | TYPE_X86_mmx              => "x86_mmx"
+    | TYPE_Array sz t           => "[" ++ show sz ++ " x " ++ show_typ t ++ "]"
+    | TYPE_Function ret args    => show_typ ret ++ " (" ++ concat ", " (map show_typ args) ++ ")"
+    | TYPE_Struct fields        => "{" ++ concat ", " (map show_typ fields) ++ "}"
+    | TYPE_Packed_struct fields => "<{" ++ concat ", " (map show_typ fields) ++ "}>"
+    | TYPE_Opaque               => "opaque"
+    | TYPE_Vector sz t          => "<" ++ show sz ++ " x " ++ show_typ t ++ ">"
+    | TYPE_Identified id        => show id
     end.
 
   Global Instance showTyp:  Show typ :=
     {|
-    show := CeresSerialize.to_string
+    show := show_typ
     |}.
+
+  Definition show_ibinop (iop : ibinop) : string
+    := match iop with
+       (* TODO print flags *)
+       | LLVMAst.Add _ _ => "add"
+       | Sub _ _ => "sub"
+       | Mul _ _ => "mul"
+       | Shl _ _ => "shl"
+       | UDiv _  => "udiv"
+       | SDiv _  => "sdiv"
+       | LShr _  => "lshr"
+       | AShr _  => "ashr"
+       | URem    => "urem"
+       | SRem    => "srem"
+       | And     => "and"
+       | Or      => "or"
+       | Xor     => "xor"
+       end.
+
+  Global Instance showIBinop : Show ibinop
+    := {| show := show_ibinop |}.
+
+  Definition show_icmp (cmp : icmp) : string
+    := match cmp with
+       | Eq  => "eq"
+       | Ne  => "ne"
+       | Ugt => "ugt"
+       | Uge => "uge"
+       | Ult => "ult"
+       | Ule => "ule"
+       | Sgt => "sgt"
+       | Sge => "sge"
+       | Slt => "slt"
+       | Sle => "sle"
+       end.
+
+  Global Instance showICmp : Show icmp
+    := {| show := show_icmp |}.
+
+  Fixpoint show_exp (v : exp typ) :=
+      match v with
+      | EXP_Ident id => show id
+      | EXP_Integer x => show x
+      | EXP_Bool b => show b
+      | EXP_Null => "null"
+      | EXP_Zero_initializer => "zero initializer"
+      | EXP_Cstring s => s (* TODO, this is probably wrong *)
+      | EXP_Undef => "undef"
+      | OP_IBinop iop t v1 v2 =>
+        show iop ++ " " ++ show t ++ " " ++ show_exp v1 ++ " " ++ show_exp v2
+      | OP_ICmp cmp t v1 v2 =>
+        show cmp ++ " " ++ show t ++ " " ++ show_exp v1 ++ " " ++ show_exp v2
+      | OP_GetElementPtr t ptrval idxs =>
+        "getelementptr"
+      | _ => "show_exp todo"
+      end.
+
+  Global Instance showExp : Show (exp typ)
+    := {| show := show_exp |}.
+
+  Global Instance showTExp : Show (texp typ)
+    := {| show te :=
+            match te with
+            | (t, e) => show t ++ " " ++ show e
+            end
+       |}.
+
+  Definition show_opt_prefix {A} `{Show A} (prefix : string) (ma : option A) : string
+    := match ma with
+       | None   => ""
+       | Some a => prefix ++ show a
+       end.
+  
+  Fixpoint show_instr (i : instr typ) : string
+    := match i with
+       | INSTR_Comment s => "; " ++ s
+       | INSTR_Op e => show e
+       | INSTR_Load vol t ptr align =>
+         "load " ++ show t ++ " " ++ show ptr ++ show_opt_prefix ", align " align
+       | INSTR_Store vol tval ptr align =>
+         "store " ++ show tval ++ " " ++ show ptr ++ show_opt_prefix ", align " align
+       | INSTR_Alloca t nb align =>
+         "alloca " ++ show t ++ show_opt_prefix ", " nb ++ show_opt_prefix ", align " align
+       | _ => "show_instr todo"
+       end.
+
+  Global Instance showInstr : Show (instr typ)
+    := {| show := show_instr |}.
+
+  Global Instance showInstrId : Show instr_id
+    := {| show i :=
+            match i with
+            | IId raw => ("%" ++ show raw)%string
+            | IVoid n => ("void<" ++ show n ++ ">")%string
+            end
+       |}.
+
+  Definition show_instr_id (inst : instr_id * instr typ) : string
+    :=
+      let '(iid, i) := inst in
+      match iid with
+        | IId _ =>
+          (show iid ++ " = " ++ show i)%string
+        | IVoid n =>
+          show i
+      end.
+
+  Global Instance showInstrWithId : Show (instr_id * instr typ)
+    := {| show := show_instr_id |}.
+
+  Definition show_terminator (t : terminator typ) : string
+    := match t with
+       | TERM_Ret v => "ret " ++ show v
+       | TERM_Ret_void => "ret"
+       | TERM_Br te b1 b2 =>
+         "br " ++ show te ++ ", label " ++ show b1 ++ ", label " ++ show b2
+       | TERM_Br_1 b =>
+         "br label " ++ show b
+       | _ => "show_terminator todo"
+       end.
+
+  Global Instance showTerminator : Show (terminator typ)
+    := {| show := show_terminator |}.
+
+  Definition show_code (indent : string) (c : code typ) : string
+    := concatStr (map (fun iid => indent ++ show_instr_id iid ++ newline) c).
+
+  Global Instance showCode : Show (code typ)
+    := {| show := show_code "    " |}.
+
+  Definition show_block (indent : string) (b : block typ) : string
+    :=
+      let code   := show_code indent (blk_code b) in
+      let term   := indent ++ show (blk_term b) ++ newline in
+      show (blk_id b) ++ ":" ++ newline
+           ++ code
+           ++ term.
 
   Global Instance showBlock: Show (block typ) :=
     {|
-    show := CeresSerialize.to_string
+    show := show_block "    "
     |}.
 
-  Global Instance showCode: Show (code typ) :=
-    {|
-    show := CeresSerialize.to_string
-    |}.
+  Definition show_arg (arg : local_id * typ) : string
+    := let '(i, t) := arg in
+       show t ++ " %" ++ show i.
 
-  Global Instance showInstr: Show (instr typ) :=
-    {|
-    show := CeresSerialize.to_string
-    |}.
+  Definition show_arg_list (args : list (local_id * typ)) : string
+    :=
+      let arg_str := concat ", " (map show_arg args) in
+      concatStr ["("; arg_str; ")"].
+
+  (* TODO: REALLY?!? *)
+  Fixpoint zip {X Y} (xs : list X) (ys : list Y) : list (X * Y)
+    := match xs, ys with
+       | [], _ => []
+       | _, [] => []
+       | (x::xs), (y::ys) => (x, y) :: zip xs ys
+       end.
+
+  Definition show_definition (defn : definition typ (list (block typ))) : string
+    :=
+      let name  := defn.(df_prototype).(dc_name) in
+      let ftype := defn.(df_prototype).(dc_type) in
+      match ftype with
+      | TYPE_Function ret_t args_t
+        =>
+        let args := zip defn.(df_args) args_t in
+        let blocks := concat newline (map (show_block "    ") (df_instrs defn)) in
+        concatStr
+          [ "define "; show ret_t; " "; show name; show_arg_list args; " {"; newline
+          ; blocks
+          ; "}"; newline
+          ]
+      | _ => "Invalid type on function: " ++ show name
+      end.
 
   Global Instance showDefinition: Show (definition typ (list (block typ))) :=
-    {|
-    show := CeresSerialize.to_string
-    |}.
+    {| show := show_definition |}.
 
-  Global Instance showExp : Show (exp typ) :=
-    {|
-    show := CeresSerialize.to_string
-    |}.
-
-  Global Instance showTexp : Show (texp typ) :=
-    {|
-    show := CeresSerialize.to_string
-    |}.
+  Definition show_tle (tle : toplevel_entity typ (list (block typ))) : string
+    := match tle with
+       | TLE_Definition defn => show_definition defn
+       | _ => "todo: show_tle"
+       end.
 
   Global Instance showTLE: Show (toplevel_entity typ (list (block typ))) :=
-    {|
-    show := CeresSerialize.to_string
-    |}.
+    {| show := show_tle |}.
+
+  Global Instance showProg : Show (list (toplevel_entity typ (list (block typ)))) :=
+    {| show tles := concat (newline ++ newline) (map show_tle tles) |}.
+
 End ShowInstances.
 
 Section Helpers.
@@ -378,6 +537,12 @@ Section GenerationState.
                   k <- lift (choose (0, n)%nat);;
                   vectorOf_LLVM k g).
 
+  Definition nonemptyListOf_LLVM
+             {A : Type} (g : GenLLVM A) : GenLLVM (list A)
+    := sized_LLVM (fun n =>
+                     k <- lift (choose (1, n)%nat);;
+                     vectorOf_LLVM k g).
+
   Definition run_GenLLVM {A} (g : GenLLVM A) : G A
     := fmap fst (runStateT g init_GenState).
 End GenerationState.
@@ -425,8 +590,8 @@ Section TypGenerators.
         ; ret TYPE_Vector <*> lift genPosZ <*> gen_sized_typ_size sz'
         ; let n := Nat.div sz 2 in
           ret TYPE_Function <*> gen_sized_typ_size n <*> listOf_LLVM (gen_sized_typ_size n)
-        ; ret TYPE_Struct <*> listOf_LLVM (gen_sized_typ_size sz')
-        ; ret TYPE_Packed_struct <*> listOf_LLVM (gen_sized_typ_size sz')
+        ; ret TYPE_Struct <*> nonemptyListOf_LLVM (gen_sized_typ_size sz')
+        ; ret TYPE_Packed_struct <*> nonemptyListOf_LLVM (gen_sized_typ_size sz')
         ]
     end.
   Next Obligation.
@@ -488,8 +653,8 @@ Section TypGenerators.
                       ; ret TYPE_Vector <*> lift genPosZ <*> gen_sized_typ_size sz'
                       ; let n := Nat.div sz 2 in
                         ret TYPE_Function <*> gen_typ_size n <*> listOf_LLVM (gen_sized_typ_size n)
-                      ; ret TYPE_Struct <*> listOf_LLVM (gen_sized_typ_size sz')
-                      ; ret TYPE_Packed_struct <*> listOf_LLVM (gen_sized_typ_size sz')
+                      ; ret TYPE_Struct <*> nonemptyListOf_LLVM (gen_sized_typ_size sz')
+                      ; ret TYPE_Packed_struct <*> nonemptyListOf_LLVM (gen_sized_typ_size sz')
                       ]
     end.
   Next Obligation.
@@ -540,8 +705,8 @@ Section TypGenerators.
                       ; ret TYPE_Vector <*> lift genPosZ <*> gen_sized_typ_size sz'
                       ; let n := Nat.div sz 2 in
                         ret TYPE_Function <*> gen_typ_size n <*> listOf_LLVM (gen_sized_typ_size n)
-                      ; ret TYPE_Struct <*> listOf_LLVM (gen_sized_typ_size sz')
-                      ; ret TYPE_Packed_struct <*> listOf_LLVM (gen_sized_typ_size sz')
+                      ; ret TYPE_Struct <*> nonemptyListOf_LLVM (gen_sized_typ_size sz')
+                      ; ret TYPE_Packed_struct <*> nonemptyListOf_LLVM (gen_sized_typ_size sz')
                       ]
     end.
 
@@ -741,7 +906,7 @@ Section ExpGenerators.
       let gen_idents :=
           match ts with
           | [] => []
-          | _ => [(4%nat, fmap (fun '(i,_) => EXP_Ident i) (oneOf_LLVM (fmap ret ts)))]
+          | _ => [(16%nat, fmap (fun '(i,_) => EXP_Ident i) (oneOf_LLVM (fmap ret ts)))]
           end in
       let gen_size_0 :=
           match t with
@@ -903,8 +1068,7 @@ Section InstrGenerators.
    *)
   Definition gen_instr : GenLLVM (typ * instr typ) :=
     oneOf_LLVM
-      [ ret (TYPE_Void, INSTR_Comment "test")
-      ; t <- gen_op_typ;; i <- ret INSTR_Op <*> gen_op t;; ret (t, i)
+      [ t <- gen_op_typ;; i <- ret INSTR_Op <*> gen_op t;; ret (t, i)
       ; t <- gen_sized_typ;;
         num_elems <- gen_opt_LLVM gen_int_texp;;
         align <- lift arbitrary;;
@@ -967,9 +1131,9 @@ Section InstrGenerators.
        | S sz' =>
          (* Need to lift oneOf to GenLLVM ...*)
          freq_LLVM
-           [ (8%nat, gen_terminator_sz 0 t)
-           ; (0%nat, '(b, bs) <- gen_blocks_sz sz' t;; ret (TERM_Br_1 (blk_id b), bs))
-           ; (0%nat, ctx <- get_ctx;;
+           [ (6%nat, gen_terminator_sz 0 t)
+           ; (min sz' 6%nat, '(b, bs) <- gen_blocks_sz sz' t;; ret (TERM_Br_1 (blk_id b), bs))
+           ; (min sz' 6%nat, ctx <- get_ctx;;
                    c <- gen_exp (TYPE_I 1);;
                    '(b1, bs1) <- gen_blocks_sz sz' t;;
 
@@ -1029,7 +1193,10 @@ Section InstrGenerators.
   Definition gen_main : GenLLVM (definition typ (list (block typ)))
     := gen_definition (Name "main") (TYPE_I 8) [].
 
-Definition gen_main_tle : GenLLVM (toplevel_entity typ (list (block typ)))
-  := ret TLE_Definition <*> gen_main.
+  Definition gen_main_tle : GenLLVM (toplevel_entity typ (list (block typ)))
+    := ret TLE_Definition <*> gen_main.
+
+  Definition gen_llvm :GenLLVM (list (toplevel_entity typ (list (block typ))))
+    := fmap ret gen_main_tle.
 
 End InstrGenerators.
