src/coq/QCVellvm.v
@@ -8,16 +8,6 @@ From ITree Require Import
      Interp.Recursion
      Events.Exception.
 
-Check TopLevelEnv.interpreter.
-Require Import Ceres.Ceres.
-
-Definition gen_llvm :GenLLVM (list (toplevel_entity typ (list (block typ))))
-  := fmap ret gen_main_tle.
-
-(* Axiom step *)
-
-Extraction gen_llvm.
-
 (* TODO: Use the existing vellvm version of this? *)
 Inductive MlResult a e :=
 | MlOk : a -> MlResult a e
@@ -38,12 +28,14 @@ Definition interpret (prog : list (toplevel_entity typ (list (block typ)))) : Ml
   := step (TopLevelEnv.interpreter prog).
 
 Definition always_zeroP (prog : list (toplevel_entity typ (list (block typ)))) : Checker
-  := match interpret prog with
-     | MlOk (UVALUE_I8 x) => collect (to_string prog) (checker true)
-     | MlError e => checker true (* Ignore errors for now *)
-     | MlOk (UVALUE_IBinop _ _ _) => collect "binop" (checker true)
-     | MlOk uv => collect (to_string uv) true
-     end.
+  := 
+    collect (show prog)
+            match interpret prog with
+            | MlOk (UVALUE_I8 x) => checker true
+            | MlError e => checker true (* Ignore errors for now *)
+            | MlOk (UVALUE_IBinop _ _ _) => checker true
+            | MlOk uv => checker true
+            end.
 
-Extract Constant defNumTests    => "100".
+Extract Constant defNumTests    => "20".
 QuickChick (forAll (run_GenLLVM gen_llvm) always_zeroP).
